Dafny/cleanup3/BloodType.dfy
@@ -1,7 +1,7 @@
 
 datatype BloodType = AP | BP | OP | ABP | AM | BM | OM | ABM
 
-predicate validBloodType(bloodType: BloodType)
+predicate method validBloodType(bloodType: BloodType)
 {
     bloodType in [AP, BP, OP, ABP, AM, BM, OM, ABM]
 }
