Dafny/cleanup3/Request.dfy
@@ -2,33 +2,3 @@
 include "BloodType.dfy"
 
 datatype Request = Request(bloodType: BloodType, volume: int)
-
-function method cumulativeVolume(req: array<Request>, upTo: int): int
-    reads req;
-    requires req != null;
-    requires 0 <= upTo <= req.Length;
-    requires forall i | 0 <= i < req.Length :: req[i].volume > 0;
-    ensures  cumulativeVolume(req, upTo) >= 0;
-{
-    if upTo == 0 then
-        0
-    else
-        req[upTo - 1].volume + cumulativeVolume(req, upTo - 1)
-}
-
-method TestCumulativeVolume()
-{
-    var req := new Request[5];
-    req[0] := Request(AP, 3);
-    req[1] := Request(BP, 1);
-    req[2] := Request(OP, 4);
-    req[3] := Request(AM, 1);
-    req[4] := Request(BM, 5);
-
-    assert cumulativeVolume(req, 0) ==  0;
-    assert cumulativeVolume(req, 1) ==  3;
-    assert cumulativeVolume(req, 2) ==  4;
-    assert cumulativeVolume(req, 3) ==  8;
-    assert cumulativeVolume(req, 4) ==  9;
-    assert cumulativeVolume(req, 5) == 14;    
-}
